More work towards ecrecover
For #17

Some of the algorithms seem to be wrong (not producing correct
results) at present.

util/recursiveLengthPrefixScript.sml
@@ -39,32 +39,6 @@ Definition dest_RLPL_def[simp]:
   dest_RLPL _ = []
 End
 
-Definition num_to_be_bytes_def:
-  num_to_be_bytes n : word8 list =
-  if n = 0 then [] else REVERSE $ MAP n2w $ n2l 256 n
-End
-
-Definition num_of_be_bytes_def:
-  num_of_be_bytes bs =
-  l2n 256 $ MAP w2n $ REVERSE bs
-End
-
-Theorem num_of_to_be_bytes[simp]:
-  num_of_be_bytes (num_to_be_bytes n) = n
-Proof
-  rw[num_of_be_bytes_def, num_to_be_bytes_def, MAP_MAP_o, o_DEF]
-  \\ qmatch_goalsub_abbrev_tac`MAP f ls`
-  \\ `MAP f ls = MAP I ls`
-  by (
-    rw[MAP_EQ_f, Abbr`ls`, Abbr`f`]
-    \\ qspec_then`256` mp_tac n2l_BOUND
-    \\ rw[EVERY_MEM]
-    \\ first_x_assum drule \\ rw[] )
-  \\ fs[Abbr`ls`]
-  \\ irule l2n_n2l
-  \\ rw[]
-QED
-
 Definition rlp_number_def:
   rlp_number n = RLPB $ num_to_be_bytes n
 End
